allocator/bitmap: Steel final implem
- extraction broken
- some admitted lemmas yet to prove

lib_bitmap/Bitmap5.fst
@@ -12,13 +12,37 @@ module A = Steel.Array
 
 let array = Steel.ST.Array.array
 
-open FStar.UInt
+module FU = FStar.UInt
 open FStar.Mul
+
+module G =  FStar.Ghost
 
 // spec is done
 // lets define the Steel implementation
 
-let bm_get
+noextract
+unfold
+let f_aux (k: nat{k < U64.n})
+  : r:nat{r < U64.n}
+  = U64.n - k - 1
+
+noextract
+unfold
+let f (#n:nat)
+  (k:nat{k < n * U64.n})
+  : r:nat{r < n * U64.n}
+  =
+  let k1 = k/U64.n in
+  let k2 = k%U64.n in
+  k1*U64.n + (f_aux k2)
+
+let f_lemma (#n: nat) (k:nat{k < n * U64.n})
+  : Lemma
+  (k / U64.n = (f #n k ) / U64.n)
+  = ()
+
+noextract
+let bm_get_aux
   (#n: nat)
   (arr: array U64.t{A.length arr = n})
   (k: U32.t{U32.v k < U64.n * n})
@@ -37,7 +61,40 @@ let bm_get
   let r = Bitmap3.get x k2 in
   return r
 
-let bm_set
+#push-options "--z3rlimit 40"
+let bm_get
+  (#n: nat)
+  (arr: array U64.t{A.length arr = n})
+  (k: U32.t{U32.v k < U64.n * n})
+  : Steel bool
+  (A.varray arr)
+  (fun _ -> A.varray arr)
+  (requires fun _ -> True)
+  (ensures fun h0 b h1 ->
+    let bm = Bitmap4.array_to_bv (A.asel arr h0) in
+    let idx = f #n (U32.v k) in
+    b = Bitmap4.get (A.asel arr h0) k /\
+    b = Seq.index bm idx /\
+    A.asel arr h1 == A.asel arr h0
+  )
+  =
+  let h = get () in
+  let s : G.erased (Seq.lseq U64.t n) = A.asel arr h in
+  let k' = f #n (U32.v k) in
+
+  let k1 = U32.div k 64ul in
+  let k2 = U32.rem k 64ul in
+  let x = A.index arr k1 in
+  let r = Bitmap3.get x k2 in
+  Bitmap3.bv_get_lemma x k2;
+  assert (r = FU.nth (U64.v (Seq.index s (U32.v k1))) (f_aux (U32.v k2)));
+  Bitmap4.array_to_bv_lemma s k';
+  assert (r = Seq.index (Bitmap4.array_to_bv s) k');
+  return r
+#pop-options
+
+noextract
+let bm_set_aux
   (#n: nat)
   (arr: array U64.t{A.length arr = n})
   (k: U32.t{U32.v k < U64.n * n})
@@ -55,7 +112,58 @@ let bm_set
   let r = Bitmap3.set x k2 in
   A.upd arr k1 r
 
-let bm_unset
+#push-options "--z3rlimit 30"
+let bm_set
+  (#n: nat)
+  (arr: array U64.t{A.length arr = n})
+  (k: U32.t{U32.v k < U64.n * n})
+  : Steel unit
+  (A.varray arr)
+  (fun _ -> A.varray arr)
+  (requires fun h0 ->
+    let bm0 = Bitmap4.array_to_bv (A.asel arr h0) in
+    let idx = f #n (U32.v k) in
+    Seq.index bm0 idx = false
+  )
+  (ensures fun h0 b h1 ->
+    let bm0 = Bitmap4.array_to_bv (A.asel arr h0) in
+    let bm1 = Bitmap4.array_to_bv (A.asel arr h1) in
+    let idx = f #n (U32.v k) in
+    A.asel arr h1 == Bitmap4.set (A.asel arr h0) k /\
+    Seq.index bm1 idx = true /\
+    bm1 == Seq.upd bm0 idx true
+  )
+  =
+  let h0 = get () in
+  let s0 : G.erased (Seq.lseq U64.t n) = A.asel arr h0 in
+  let k' = f #n (U32.v k) in
+  let k1 = U32.div k 64ul in
+  let k2 = U32.rem k 64ul in
+  let x = A.index arr k1 in
+  Bitmap4.array_to_bv_lemma s0 k';
+  assert (Seq.index (Bitmap4.array_to_bv s0) k' = false);
+  assert (U32.v k1 = U32.v k / 64);
+  f_lemma #n (U32.v k);
+  assert (k' / U64.n = U32.v k1);
+  let r = Bitmap3.set x k2 in
+  Bitmap3.bv_set_lemma x k2;
+  A.upd arr k1 r;
+
+  let h1 = get () in
+  let s1 : G.erased (Seq.lseq U64.t n) = A.asel arr h1 in
+  Bitmap4.array_to_bv_lemma s1 k';
+  assert (Seq.index (Bitmap4.array_to_bv s1) k' = true);
+  assert (G.reveal s1 == Seq.upd s0 (U32.v k1) r);
+  let bm0 = Bitmap4.array_to_bv s0 in
+  let bm1 = Bitmap4.array_to_bv s1 in
+  Bitmap4.array_to_bv_lemma_upd_set
+    #n
+    s0 s1 (U32.v k);
+  Seq.lemma_eq_intro bm1 (Seq.upd bm0 k' true)
+#pop-options
+
+noextract
+let bm_unset_aux
   (#n: nat)
   (arr: array U64.t{A.length arr = n})
   (k: U32.t{U32.v k < U64.n * n})
@@ -73,6 +181,52 @@ let bm_unset
   let r = Bitmap3.unset x k2 in
   A.upd arr k1 r
 
-// additional versions with refined spec
-// use get/set/unset_lemma
-// use array_to_bv
+#push-options "--z3rlimit 30"
+let bm_unset
+  (#n: nat)
+  (arr: array U64.t{A.length arr = n})
+  (k: U32.t{U32.v k < U64.n * n})
+  : Steel unit
+  (A.varray arr)
+  (fun _ -> A.varray arr)
+  (requires fun h0 ->
+    let bm0 = Bitmap4.array_to_bv (A.asel arr h0) in
+    let idx = f #n (U32.v k) in
+    Seq.index bm0 idx = true
+  )
+  (ensures fun h0 b h1 ->
+    let bm0 = Bitmap4.array_to_bv (A.asel arr h0) in
+    let bm1 = Bitmap4.array_to_bv (A.asel arr h1) in
+    let idx = f #n (U32.v k) in
+    A.asel arr h1 == Bitmap4.unset (A.asel arr h0) k /\
+    Seq.index bm1 idx = false /\
+    bm1 == Seq.upd bm0 idx false
+  )
+  =
+  let h0 = get () in
+  let s0 : G.erased (Seq.lseq U64.t n) = A.asel arr h0 in
+  let k' = f #n (U32.v k) in
+  let k1 = U32.div k 64ul in
+  let k2 = U32.rem k 64ul in
+  let x = A.index arr k1 in
+  Bitmap4.array_to_bv_lemma s0 k';
+  assert (Seq.index (Bitmap4.array_to_bv s0) k' = true);
+  assert (U32.v k1 = U32.v k / 64);
+  f_lemma #n (U32.v k);
+  assert (k' / U64.n = U32.v k1);
+  let r = Bitmap3.unset x k2 in
+  Bitmap3.bv_unset_lemma x k2;
+  A.upd arr k1 r;
+
+  let h1 = get () in
+  let s1 : G.erased (Seq.lseq U64.t n) = A.asel arr h1 in
+  Bitmap4.array_to_bv_lemma s1 k';
+  assert (Seq.index (Bitmap4.array_to_bv s1) k' = false);
+  assert (G.reveal s1 == Seq.upd s0 (U32.v k1) r);
+  let bm0 = Bitmap4.array_to_bv s0 in
+  let bm1 = Bitmap4.array_to_bv s1 in
+  Bitmap4.array_to_bv_lemma_upd_unset
+    #n
+    s0 s1 (U32.v k);
+  Seq.lemma_eq_intro bm1 (Seq.upd bm0 k' false)
+#pop-options
